HoareLc_woc.v
@@ -5,7 +5,7 @@ Require Import Hoare_woc.
 
 
 Definition LContSet := list (label * Assertion).
-
+Print ceval'.
 Definition hoare_triple' (fc : func_context) (P : LContSet) (c : com) (Q : LContSet) : Prop :=
   forall st1 st2 l1 l2 p q,
     In (l1, p) P ->
@@ -14,5 +14,16 @@ Definition hoare_triple' (fc : func_context) (P : LContSet) (c : com) (Q : LCont
     p st1 ->
     q st2.
 
+Definition bridge_between_hoares_re : Prop :=
+  forall fc lf f' l1 l2 I,
+  In f' lf ->
+  hoare_triple' fc ((l1, I) :: nil) (snd (fc f')) ((l2, I) :: nil) ->
+  hoare_triple fc I (CReentry lf) I.
 
+Theorem bridge_between_hoares_re_correct : bridge_between_hoares_re.
+Proof.
+  unfold bridge_between_hoares_re, hoare_triple', hoare_triple.
+  intros.
+Admitted.
 
+Definition bridge_between_hoares_func : Prop
